Cpc/Proofs/Translation/Special.lean
@@ -10,6 +10,8 @@ set_option maxHeartbeats 10000000
 
 namespace TranslationProofs
 
+variable [TranslationBridge]
+
 /-- Simplifies EO-to-SMT translation for `typeof_matches_translation_purify`. -/
 theorem eo_to_smt_typeof_matches_translation_purify
     (x : Term)
